bijectivity lemma for little_endian

code/lib/FStar.Endianness.fst
@@ -1,9 +1,5 @@
 module FStar.Endianness
 
-module ST = FStar.HyperStack.ST
-
-open FStar.HyperStack.All
-
 open FStar.UInt32
 open FStar.Ghost
 open FStar.Mul
@@ -41,8 +37,8 @@ let rec little_endian (b:bytes) : Tot (n:nat) (decreases (Seq.length b)) =
     UInt8.v (head b) + pow2 8 * little_endian (tail b)
 
 (* Big endian integer value of a sequence of bytes *)
-let rec big_endian (b:bytes) : Tot (n:nat) (decreases (Seq.length b)) = 
-  if Seq.length b = 0 then 0 
+let rec big_endian (b:bytes) : Tot (n:nat) (decreases (Seq.length b)) =
+  if Seq.length b = 0 then 0
   else
     UInt8.v (last b) + pow2 8 * big_endian (Seq.slice b 0 (Seq.length b - 1))
 
@@ -55,7 +51,7 @@ let rec little_endian_null len =
   else
     begin
     Seq.lemma_eq_intro (Seq.slice (Seq.create len 0uy) 1 len)
-		       (Seq.create (len - 1) 0uy);
+           (Seq.create (len - 1) 0uy);
     assert (little_endian (Seq.create len 0uy) ==
       0 + pow2 8 * little_endian (Seq.slice (Seq.create len 0uy) 1 len));
     little_endian_null (len - 1)
@@ -182,16 +178,16 @@ let uint8_to_uint128 a = FStar.UInt128.uint64_to_uint128 (uint8_to_uint64 a)
 
 
 // turns an integer into a bytestream, little-endian
-val little_bytes: 
+val little_bytes:
   len:UInt32.t -> n:nat{n < pow2 (8 * v len)} ->
   Tot (b:lbytes (v len) {n == little_endian b}) (decreases (v len))
-let rec little_bytes len n = 
-  if len = 0ul then 
-    Seq.createEmpty 
+let rec little_bytes len n =
+  if len = 0ul then
+    Seq.createEmpty
   else
-    let len = len -^ 1ul in 
+    let len = len -^ 1ul in
     let byte = UInt8.uint_to_t (n % 256) in
-    let n' = n / 256 in 
+    let n' = n / 256 in
     Math.Lemmas.pow2_plus 8 (8 * v len);
     assert(n' < pow2 (8 * v len ));
     let b' = little_bytes len n' in
@@ -202,7 +198,7 @@ let rec little_bytes len n =
 #reset-options "--initial_fuel 1 --max_fuel 1 --initial_ifuel 0 --max_ifuel 0"
 
 
-(* injectivity proofs for byte encodings *) 
+(* injectivity proofs for byte encodings *)
 
 type word = b:Seq.seq UInt8.t {Seq.length b <= 16}
 open FStar.Math.Lib
@@ -213,7 +209,7 @@ private let endian_is_injective q r q' r' : Lemma
   (ensures r = r' /\ q = q') =
   lemma_mod_injective (pow2 8) (UInt8.v r) (UInt8.v r')
 
-private let big_endian_step (b:word{length b > 0}) : 
+private let big_endian_step (b:word{length b > 0}) :
   Lemma (big_endian b = U8.v (last b) + pow2 8 * big_endian (slice b 0 (length b - 1))) =
   ()
 
@@ -222,16 +218,16 @@ val lemma_big_endian_inj: b:word -> b':word {length b = length b'} -> Lemma
   (requires big_endian b = big_endian b')
   (ensures b == b')
   (decreases (length b))
-let rec lemma_big_endian_inj s s' = 
-  let len = length s in 
+let rec lemma_big_endian_inj s s' =
+  let len = length s in
   if len = 0 then lemma_eq_intro s s'
   else
-    let t = slice s 0 (len - 1) in 
-    let x = last s in 
+    let t = slice s 0 (len - 1) in
+    let x = last s in
     lemma_eq_intro s (snoc t x);
     big_endian_step s;
-    let t' = slice s' 0 (len - 1) in 
-    let x' = last s' in 
+    let t' = slice s' 0 (len - 1) in
+    let x' = last s' in
     lemma_eq_intro s' (snoc t' x');
     big_endian_step s';
     endian_is_injective (big_endian t) x (big_endian t') x';
@@ -250,7 +246,7 @@ let lemma_little_endian_is_injective_1 b q r q' r' =
 
 (* a sequence associativity property: ... @ ([x] @ s) == ... @ [x]) @ s *)
 private val lemma_little_endian_is_injective_2: b:bytes -> len:pos{len <= length b} -> Lemma
-  (let s = slice b (length b - len) (length b) in 
+  (let s = slice b (length b - len) (length b) in
    let s' = slice s 1 (length s) in
    let s'' = slice b (length b - (len - 1)) (length b) in
    s'' == s')
@@ -262,16 +258,16 @@ let lemma_little_endian_is_injective_2 b len =
 
 (* a sequence injectivity property *)
 private val lemma_little_endian_is_injective_3: b:bytes -> b':bytes -> len:pos{len <= length b /\ len <= length b'} -> Lemma
-  (requires 
-    slice b (length b - (len - 1)) (length b) == slice b' (length b' - (len-1)) (length b') /\ 
+  (requires
+    slice b (length b - (len - 1)) (length b) == slice b' (length b' - (len-1)) (length b') /\
     Seq.index b (length b - len) = Seq.index b' (length b' - len))
   (ensures slice b (length b - len) (length b) == slice b' (length b' - len) (length b'))
 let lemma_little_endian_is_injective_3 b b' len =
   lemma_eq_intro (slice b (length b - len) (length b)) (cons (index b (length b - len)) (slice b (length b - (len-1)) (length b)));
   lemma_eq_intro (slice b' (length b' - len) (length b')) (cons (index b' (length b' - len)) (slice b' (length b' - (len-1)) (length b')))
 
-private let little_endian_step (b:bytes{length b > 0}): 
-  Lemma (little_endian b = U8.v (head b) + pow2 8 * little_endian (tail b)) 
+private let little_endian_step (b:bytes{length b > 0}):
+  Lemma (little_endian b = U8.v (head b) + pow2 8 * little_endian (tail b))
   = ()
 
 val lemma_little_endian_is_injective: b:bytes -> b':bytes -> len:nat{len <= length b /\ len <= length b'} -> Lemma
@@ -283,7 +279,7 @@ let rec lemma_little_endian_is_injective b b' len =
   else
     let s = slice b (length b - len) (length b) in
     let s' = slice b' (length b' - len) (length b') in
-    little_endian_step s; 
+    little_endian_step s;
     little_endian_step s';
     endian_is_injective (little_endian (tail s)) (head s) (little_endian (tail s')) (head s');
     lemma_little_endian_is_injective_2 b len;
@@ -293,69 +289,78 @@ let rec lemma_little_endian_is_injective b b' len =
 
 val lemma_little_endian_inj: b:bytes -> b':bytes {length b = length b'} -> Lemma
   (requires little_endian b = little_endian b')
-  (ensures b == b')
+  (ensures b = b')
 let lemma_little_endian_inj b b' =
-  let len = length b in 
+  let len = length b in
   Seq.lemma_eq_intro b (Seq.slice b 0  len);
   Seq.lemma_eq_intro b' (Seq.slice b' 0  len);
   lemma_little_endian_is_injective b b' len
 
 
-val uint32_bytes: 
-  len:UInt32.t {v len <= 4} -> n:UInt32.t {UInt32.v n < pow2 (8 * v len)} -> 
+val lemma_little_endian_bij: b:bytes -> b':bytes{Seq.length b = Seq.length b'} -> Lemma
+  (requires True)
+  (ensures little_endian b = little_endian b' <==> b = b' )
+let lemma_little_endian_bij b b' =
+  if little_endian b = little_endian b' then
+    lemma_little_endian_inj b b'
+  else
+    ()
+
+val uint32_bytes:
+  len:UInt32.t {v len <= 4} -> n:UInt32.t {UInt32.v n < pow2 (8 * v len)} ->
   Tot (b:lbytes (v len) { UInt32.v n == little_endian b}) (decreases (v len))
-let rec uint32_bytes len n = 
-  if len = 0ul then 
+let rec uint32_bytes len n =
+  if len = 0ul then
     let e = Seq.createEmpty #UInt8.t in
     assert_norm(0 = little_endian e);
     e
   else
-    let len = len -^ 1ul in 
+    let len = len -^ 1ul in
     let byte = uint32_to_uint8 n in
     let n1 = n in (* n defined in FStar.UInt32, so was shadowed, so renamed into n1 *)
-    let n' = FStar.UInt32.(n1 >>^ 8ul) in 
+    let n' = FStar.UInt32.(n1 >>^ 8ul) in
     assert(v n = UInt8.v byte + 256 * v n');
     Math.Lemmas.pow2_plus 8 (8 * v len);
     assert_norm (pow2 8 == 256);
     assert(v n' < pow2 (8 * v len ));
     let b' = uint32_bytes len n'
-    in 
+    in
     Seq.cons byte b'
 
-val uint32_be: 
-  len:UInt32.t {v len <= 4} -> n:UInt32.t {UInt32.v n < pow2 (8 * v len)} -> 
+val uint32_be:
+  len:UInt32.t {v len <= 4} -> n:UInt32.t {UInt32.v n < pow2 (8 * v len)} ->
   Tot (b:lbytes (v len) { UInt32.v n == big_endian b}) (decreases (v len))
-let rec uint32_be len n = 
-  if len = 0ul then 
+let rec uint32_be len n =
+  if len = 0ul then
     let e = Seq.createEmpty #UInt8.t in
     assert_norm(0 = big_endian e);
     e
   else
-    let len = len -^ 1ul in 
+    let len = len -^ 1ul in
     let byte = uint32_to_uint8 n in
     let n1 = n in (* n shadowed by FStar.UInt32.n *)
-    let n' = FStar.UInt32.(n1 >>^ 8ul) in 
+    let n' = FStar.UInt32.(n1 >>^ 8ul) in
     assert(v n = UInt8.v byte + 256 * v n');
     Math.Lemmas.pow2_plus 8 (8 * v len);
     assert_norm (pow2 8 == 256);
     assert(v n' < pow2 (8 * v len ));
     let b' = uint32_be len n'
-    in 
-    Seq.snoc b' byte 
+    in
+    Seq.snoc b' byte
 
 #reset-options "--z3rlimit 400"
 
 // turns an integer into a bytestream, big-endian
-val big_bytes: 
+val big_bytes:
   len:UInt32.t -> n:nat{n < pow2 (8 * v len)} ->
   Tot (b:lbytes (v len) {n == big_endian b}) (decreases (v len))
-let rec big_bytes len n = 
-  if len = 0ul then 
-    Seq.createEmpty 
+let rec big_bytes len n =
+  if len = 0ul then
+    Seq.createEmpty
   else
-    let len = len -^ 1ul in 
+    let len = len -^ 1ul in
     let byte = UInt8.uint_to_t (n % 256) in
-    let n' = n / 256 in 
+    let n' = n / 256 in
     Math.Lemmas.pow2_plus 8 (8 * v len);
     assert(n' < pow2 (8 * v len ));
     let b' = big_bytes len n' in
